Allow heaplets to be non-ghost

vale/specs/hardware/Vale.Arch.HeapTypes_s.fst
@@ -19,18 +19,20 @@ let machine_heap = Map.t int nat8
 let memTaint_t = (m:Map.t int taint{Set.equal (Map.domain m) (Set.complement Set.empty)})
 let heaplet_id = n:nat{n < 16}
 
-let heaplets8 (ptr:int) (k:heaplet_id) (m:option (int -> option heaplet_id)) : bool =
-  match m with None -> true | Some d -> d ptr = Some k
+let t_heaplet_domains = (int -> option heaplet_id) & (heaplet_id -> Set.set int)
 
-let heaplets16 (ptr:int) (k:heaplet_id) (m:option (int -> option heaplet_id)) : bool =
+let heaplets8 (ptr:int) (k:heaplet_id) (m:option t_heaplet_domains) : bool =
+  match m with None -> true | Some (d, _) -> d ptr = Some k
+
+let heaplets16 (ptr:int) (k:heaplet_id) (m:option t_heaplet_domains) : bool =
   heaplets8 ptr k m && heaplets8 (ptr + 1) k m 
 
-let heaplets32 (ptr:int) (k:heaplet_id) (m:option (int -> option heaplet_id)) : bool =
+let heaplets32 (ptr:int) (k:heaplet_id) (m:option t_heaplet_domains) : bool =
   heaplets16 ptr k m && heaplets16 (ptr + 2) k m 
 
 [@"opaque_to_smt"]
-let heaplets64 (ptr:int) (k:heaplet_id) (m:option (int -> option heaplet_id)) : bool =
+let heaplets64 (ptr:int) (k:heaplet_id) (m:option t_heaplet_domains) : bool =
   heaplets32 ptr k m && heaplets32 (ptr + 4) k m 
 
-let heaplets128 (ptr:int) (k:heaplet_id) (m:option (int -> option heaplet_id)) : bool =
+let heaplets128 (ptr:int) (k:heaplet_id) (m:option t_heaplet_domains) : bool =
   heaplets64 ptr k m && heaplets64 (ptr + 8) k m 
