vale/code/arch/Vale.Arch.HeapImpl.fsti
@@ -32,7 +32,7 @@ val vale_heap_layout_inner : Type u#1
 noeq type vale_heap_layout : Type u#1 = {
   vl_inner:vale_heap_layout_inner;
   vl_taint:memTaint_t;
-  vl_heaplet_domains:option (int -> option heaplet_id); // for reordering transformer, non-ghost version of vl_inner.vl_heaplet_map
+  vl_heaplet_domains:option t_heaplet_domains; // for reordering transformer, non-ghost version of vl_inner.vl_heaplet_map and vl_inner.vl_heaplet_sets
 }
 
 let vale_heaplets = Map16.map16 vale_heap
